simplify transition systems

src/Transition.v
@@ -9,38 +9,6 @@ Import ListNotations.
 
 Require Import CrossCrypto.Tail.
 
-Definition head T (l : list T) (H : l <> []) : T.
-  destruct l.
-  destruct (H eq_refl).
-  exact t.
-Defined.
-
-Inductive rosetree (T : Type) : Type :=
-| RLeaf : rosetree T
-| RNode : T -> list (rosetree T) -> rosetree T.
-
-Arguments RLeaf {T}.
-
-Definition rosetree_list_rect (T : Type)
-           (P : rosetree T -> Type)
-           (Q : list (rosetree T) -> Type)
-           (p_leaf : P RLeaf)
-           (p_node : forall x l, Q l -> P (RNode x l))
-           (q_nil : Q [])
-           (q_cons : forall r l, P r -> Q l -> Q (r :: l)) :
-  forall r : rosetree T, P r :=
-  fix F (r : rosetree T) : P r :=
-  match r with
-    | RLeaf => p_leaf
-    | RNode x l =>
-      p_node x l
-             ((fix G (l : list (rosetree T)) : Q l :=
-                 match l with
-                   | [] => q_nil
-                   | r :: l => q_cons r l (F r) (G l)
-                 end) l)
-  end.
-
 Inductive eq_2 (A : Type) (P : A -> Type) (a a' : A) (p : P a) (p' : P a')
 : Prop :=
 | eq_refl2 : forall (H : a = a'),
@@ -63,135 +31,67 @@ Section Protocols.
 
   Variable input : Type.
 
-  Section Protocol.
-
-    Variable state : Type.
-    Variable initial : state.
-    Variable state_lt : state -> state -> Prop.
-    Variable state_wf : well_founded state_lt.
-
-    Variable transition : state -> Type.
-    Variable transition_guard : forall q, transition q -> input -> Prop.
-    Variable transition_update : forall q (t : transition q), input -> state.
-    Variable transition_next_lt : forall q (t : transition q) i,
-                                    state_lt (@transition_update _ t i) q.
-
-    Variable transition_lt : forall q, transition q -> transition q -> Prop.
-
-    Variable transition_lt_total :
-      forall q (t t' : transition q),
-         t = t' \/ transition_lt t t' \/ transition_lt t' t.
-
-    Definition final_ q := transition q -> False.
-
-    Definition maximal_transition q (t : transition q) :=
-      forall i, transition_guard t i.
-
-    Definition has_max_transition q (H : ~final_ q) : Prop :=
-      exists t : transition q, maximal_transition t.
-
-  End Protocol.
-
   Record protocol :=
     mkProtocol {
         state : Type;
         initial : state;
         state_lt : state -> state -> Prop;
         state_wf : well_founded state_lt;
-        transition : state -> Type;
-        transition_guard : forall q, transition q -> input -> Prop;
-        transition_update : forall q (t : transition q), input -> state;
-        transition_next_lt : forall q (t : transition q) i,
-                               state_lt (@transition_update _ t i) q;
-
-        transition_lt : forall q, transition q -> transition q -> Prop;
-        transition_lt_total :
-          forall q (t t' : transition q),
-            t = t' \/ transition_lt t t' \/ transition_lt t' t;
-        final : state -> Prop := final_ transition;
-        max_transition : forall q (H : ~final q),
-                           has_max_transition transition_guard H;
       }.
 
-  Definition valid_transition p (q : p.(state))
-             (t : transition q) (i : input) :=
-    transition_guard t i /\
-    forall t', transition_lt t t' -> ~transition_guard t' i.
+  Definition final p (q : p.(state)) :=
+    forall q', ~state_lt q' q.
 
-  Lemma valid_transition_unique p (q : p.(state))
-        (t t' : transition q) (i : input) :
-    valid_transition t i -> valid_transition t' i -> t = t'.
-    intros Vt Vt'.
-    destruct (transition_lt_total t t') as [e | [lt | lt]];
-      [assumption | ..];
-      destruct Vt as [Vt nVt'];
-      destruct Vt' as [Vt' nVt];
-      [destruct (nVt' t' lt Vt') | destruct (nVt t lt Vt)].
-  Qed.
+  Definition unique_transition p :=
+    forall q q' q'': p.(state),
+      state_lt q' q -> state_lt q'' q -> q' = q''.
 
-  Definition client p := p.(state) -> input.
-
-  Definition valid_transition_client p (c : p.(client)) q (t : transition q) :=
-    valid_transition t (c q).
-
-  Definition valid_transition_unique_client p (c : p.(client)) q
-             (t t' : transition q)
-             (Vt : valid_transition_client c t)
-             (Vt' : valid_transition_client c t') : t = t' :=
-    valid_transition_unique Vt Vt'.
-
-
-  Definition transition_update_client p (c : p.(client)) q
-             (t : transition q) :=
-    transition_update t (c q).
+  Definition transition_dec p :=
+    forall q : p.(state), {q' : p.(state) & state_lt q' q} + {final q}.
 
   (* TODO use more traditional semantics style than these traces *)
 
-  Inductive reaches p (c : client p) : p.(state) -> Type :=
-  | RInitial : reaches c p.(initial)
-  | RTransition : forall q (t : transition q)
-                         (Hv : valid_transition_client c t),
-                    reaches c q -> reaches c (transition_update_client c t).
+  Inductive reaches p : p.(state) -> Type :=
+  | RInitial : reaches p.(initial)
+  | RTransition : forall q q' (t : state_lt q' q),
+                    reaches q -> reaches q'.
 
-  Fixpoint reaches_n p (c : client p) q (R : reaches c q) : nat :=
+  Fixpoint reaches_n p (q : p.(state)) (R : reaches q) : nat :=
     match R with
       | RInitial _ => O
-      | @RTransition _ _ q' _ _ R => S (@reaches_n p c q' R)
+      | @RTransition _ q' _ _ R => S (@reaches_n p q' R)
     end.
 
-  Lemma root_unique p (c : client p) q (R : reaches c q) :
+  Lemma root_unique p (q : p.(state)) (R : reaches q) :
     reaches_n R = 0 -> q = p.(initial).
     intro H.
     induction R.
     reflexivity.
-    simpl in H; congruence.
+    simpl in H; discriminate.
   Qed.
 
-  Lemma reaches_n_inv p (c : client p) q (R : reaches c q) n :
+  Lemma reaches_n_inv p (q : p.(state)) (R : reaches q) n :
     reaches_n R = S n ->
-    exists q' (t : transition q') (Hv : valid_transition_client c t)
-           (R' : reaches c q'),
-      (eq_2 R (RTransition Hv R')) /\ reaches_n R' = n.
+    exists q' (t : state_lt q q') (R' : reaches q'),
+      R = (RTransition t R') /\ reaches_n R' = n.
     intro H.
     revert n H.
     remember R as r.
-    destruct r as [| q t Hv r]; intros n H.
+    destruct r as [| q' q H0 r]; intros n H.
     inversion H.
-    exists q.
-    exists t.
-    exists Hv.
+
+    exists q'.
+    exists H0.
     exists r.
     split.
-    apply eq_refl2 with (H := eq_refl).
-    simpl.
     reflexivity.
-    simpl in H.
+
     inversion H.
     reflexivity.
   Qed.
 
-  Lemma reaches_unique_n p (c : client p) q q'
-        (R : reaches c q) (R' : reaches c q') :
+  Lemma reaches_unique_n p (U : unique_transition p) (q q' : p.(state))
+        (R : reaches q) (R' : reaches q') :
     reaches_n R = reaches_n R' -> q = q'.
     remember (reaches_n R) as n eqn:HnR.
     intro HnR'.
@@ -204,68 +104,91 @@ Section Protocols.
     pose proof (reaches_n_inv HnR) as H.
     pose proof (reaches_n_inv HnR') as H'.
     clear HnR HnR'.
-    destruct H as [q0 [t0 [Hv0 [R0 [[? eR] HnR0]]]]].
-    subst q.
-    simpl in eR.
+    destruct H as [q0 [? [? [? ?]]]].
     subst R.
 
-    destruct H' as [q0' [t0' [Hv0' [R0' [[? eR'] HnR0']]]]].
-    subst q'.
-    simpl in eR'.
+    destruct H' as [q0' [? [? [? ?]]]].
     subst R'.
 
     assert (q0 = q0') by (eapply IHn; eassumption).
     subst q0'.
-    assert (t0 = t0') by (eapply valid_transition_unique_client; eassumption).
-    subst t0'.
-    reflexivity.
+
+    eapply U; eassumption.
   Qed.
 
-  Lemma no_final_extension p (c : client p) q q'
-        (R : reaches c q) (R' : reaches c q') :
+  Lemma no_final_greater p (U : unique_transition p) (q q' : p.(state))
+        (R : reaches q) (R' : reaches q') :
     final q -> reaches_n R < reaches_n R' -> False.
     intros Fq l.
 
     assert (exists n, reaches_n R' = S (n + reaches_n R)) as l' by
           (exists (reaches_n R' - reaches_n R - 1); omega); clear l.
     destruct l' as [n H].
-    destruct (reaches_n_inv H) as [q'0 [t [Hv [R'0 [[? _] HnR'0]]]]];
-      clear H.
-    subst q'.
-    clear R'.
+    destruct (reaches_n_inv H) as [q'0 [t'0 [R'0 [_ HnR'0]]]]; clear H R'.
 
-    revert q R Fq q'0 t Hv R'0 HnR'0.
-    induction n; intros q R Fq q'0 t Hv R'0 HnR'0.
+    revert q' q'0 t'0 R'0 HnR'0.
+    induction n; intros q' q'0 t'0 R'0 HnR'0.
 
     simpl in HnR'0.
     assert (q = q'0) by
         (symmetry in HnR'0; eapply reaches_unique_n; eassumption).
     subst q'0.
-    exact (Fq t).
+    eapply Fq; eassumption.
 
-    destruct (reaches_n_inv HnR'0) as [q'1 [t0 [Hv0 [R'1 [[? _] HnR'1]]]]];
-      clear HnR'0.
-    subst q'0.
-    clear R'0.
+    destruct (reaches_n_inv HnR'0) as [q'1 [t'1 [R'1 [_ HnR'1]]]].
+    clear HnR'0 R'0.
 
-    eapply IHn with (t:=t0); eassumption.
+    eapply IHn; swap 1 2; eassumption.
   Qed.
 
-  Lemma reaches_unique_final_n p (c : client p) q q' (R : reaches c q)
-        (R' : reaches c q') :
+  Lemma reaches_unique_final_n p (U : unique_transition p)
+        (q q' : p.(state)) (R : reaches q)
+        (R' : reaches q') :
     final q -> final q' -> reaches_n R = reaches_n R'.
     intros Fq Fq'.
     destruct (lt_eq_lt_dec (reaches_n R) (reaches_n R')) as [[l | e] | l];
       [exfalso | assumption | exfalso];
-      eapply no_final_extension; swap 1 2; eassumption.
+      eapply no_final_greater; swap 2 3; eassumption.
   Qed.
 
-  Theorem reaches_unique_final p (c : client p) q q'
-          (R : reaches c q) (R' : reaches c q') :
+  Theorem reaches_unique_final p (U : unique_transition p) (q q' : p.(state))
+          (R : reaches q) (R' : reaches q') :
     final q -> final q' -> q = q'.
     intros Fq Fq'.
-    apply reaches_unique_n with (c:=c) (R:=R) (R':=R');
-    apply reaches_unique_final_n; assumption.
+    eapply reaches_unique_n with (R := R) (R' := R');
+      [assumption | eapply reaches_unique_final_n; eassumption].
   Qed.
+
+
+  Definition extend_reach p (E : transition_dec p) (q : p.(state))
+             (R : reaches q) :
+    {q' : p.(state) & (reaches q') * state_lt q' q}%type + {final q}.
+    destruct (E q) as [[q' t] | Fq].
+    left; exists q'; split; [econstructor|]; eassumption.
+    right; assumption.
+  Defined.
+
+  Definition finalize_reach p (E : transition_dec p) (q : p.(state))
+             (R : reaches q) :
+    {q' : p.(state) & (reaches q') * (final q')}%type.
+    revert q R.
+    refine
+      (Fix p.(@state_wf)
+               (fun q : p.(state) =>
+                  reaches (p:=p) q ->
+                  {q' : state p &
+                        (reaches (p:=p) q' * final (p:=p) q')%type}) _).
+    intros q IHq R.
+    destruct (E q) as [[q' t] | Fq].
+    eapply IHq; [|econstructor]; eassumption.
+
+    exists q.
+    split; assumption.
+  Defined.
+
+  Definition exists_reaches p (E : transition_dec p) :
+    {q : p.(state) & (reaches q) * (final q)}%type.
+    eapply finalize_reach; [assumption | constructor].
+  Defined.
 
 End Protocols.
